compiler/backend/semantics/flatPropsScript.sml
@@ -323,6 +323,14 @@ Proof
   \\ rpt (pairarg_tac \\ gvs [])
 QED
 
+Theorem do_app_ptr_eq_oracle:
+  !s op vs s' r. do_app s op vs = SOME (s', r) ∧ op ≠ Src PtrEq ⇒
+     s'.ptr_eq_oracle = s.ptr_eq_oracle
+Proof
+  rw [do_app_def,AllCaseEqs()] \\ gvs []
+  \\ rpt (pairarg_tac \\ gvs [])
+QED
+
 Theorem evaluate_decs_append:
   !s ds1 s1 s2 r ds2.
     evaluate_decs s (ds1++ds2) =
@@ -617,8 +625,8 @@ QED
 
 Theorem evaluate_decs_add_to_clock_initial_state[local]:
   r ≠ SOME (Rabort Rtimeout_error) ∧
-   evaluate_decs (initial_state ffi k ec) decs = (s',r) ⇒
-   evaluate_decs (initial_state ffi (ck + k) ec) decs =
+   evaluate_decs (initial_state ffi k ec pe) decs = (s',r) ⇒
+   evaluate_decs (initial_state ffi (ck + k) ec pe) decs =
    (s' with clock := s'.clock + ck,r)
 Proof
   rw [initial_state_def]
@@ -626,9 +634,9 @@ Proof
 QED
 
 Theorem evaluate_decs_add_to_clock_initial_state_io_events_mono[local]:
-  evaluate_decs (initial_state ffi k ec) prog = (s',r) ==>
+  evaluate_decs (initial_state ffi k ec pe) prog = (s',r) ==>
    s'.ffi.io_events ≼
-   (FST (evaluate_decs (initial_state ffi (k+ck) ec) prog)).ffi.io_events
+   (FST (evaluate_decs (initial_state ffi (k+ck) ec pe) prog)).ffi.io_events
 Proof
   rw [initial_state_def]
   \\ qmatch_assum_abbrev_tac `evaluate_decs s1 _ = _`
@@ -639,8 +647,8 @@ Proof
 QED
 
 Theorem initial_state_with_clock[local]:
-  (initial_state ffi k ec with clock := (initial_state ffi k ec).clock + ck) =
-   initial_state ffi (k + ck) ec
+  (initial_state ffi k ec pe with clock := (initial_state ffi k ec pe).clock + ck) =
+   initial_state ffi (k + ck) ec pe
 Proof
   rw [initial_state_def]
 QED
@@ -652,15 +660,15 @@ Proof
 QED
 
 Definition eval_sim_def:
-  eval_sim ffi ds1 ds2 ec ec2 rel allow_fail =
+  eval_sim ffi pe ds1 ds2 ec ec2 rel allow_fail =
     !k res1 s2.
-      evaluate_decs (initial_state ffi k ec) ds1 =
+      evaluate_decs (initial_state ffi k ec pe) ds1 =
         (s2, res1) /\
       (allow_fail \/ res1 <> SOME (Rabort Rtype_error)) /\
       rel ds1 ds2
       ==>
       ?ck res2 t2.
-        evaluate_decs (initial_state ffi (k + ck) ec2) ds2 =
+        evaluate_decs (initial_state ffi (k + ck) ec2 pe) ds2 =
           (t2, res2) /\
         s2.ffi = t2.ffi /\
         (res1 = NONE ==> res2 = NONE) /\
@@ -669,11 +677,11 @@ Definition eval_sim_def:
 End
 
 Theorem IMP_semantics_eq:
-   eval_sim ffi ds1 ds2 ec ec2 rel F /\
-   semantics ec (ffi:'ffi ffi_state) ds1 <> Fail ==>
+   eval_sim ffi pe ds1 ds2 ec ec2 rel F /\
+   semantics ec (ffi:'ffi ffi_state) pe ds1 <> Fail ==>
    rel ds1 ds2 ==>
-   semantics ec ffi ds1 =
-   semantics ec2 ffi ds2
+   semantics ec ffi pe ds1 =
+   semantics ec2 ffi pe ds2
 Proof
   rewrite_tac [GSYM AND_IMP_INTRO]
   \\ strip_tac
@@ -727,7 +735,7 @@ Proof
   \\ simp [Once semantics_def]
   \\ IF_CASES_TAC \\ fs [SND_SND_lemma]
   >-
-   (`?a b. evaluate_decs (initial_state ffi k ec) ds1 = (a,b)`
+   (`?a b. evaluate_decs (initial_state ffi k ec pe) ds1 = (a,b)`
         by simp [PAIR_FST_SND_EQ]
     \\ first_x_assum (qspec_then `k` mp_tac)
     \\ simp []
@@ -741,7 +749,7 @@ Proof
   \\ DEEP_INTRO_TAC some_intro
   \\ fs [] \\ rw []
   >-
-   (`?a b. evaluate_decs (initial_state ffi k ec) ds1 = (a,b)`
+   (`?a b. evaluate_decs (initial_state ffi k ec pe) ds1 = (a,b)`
         by simp [PAIR_FST_SND_EQ]
     \\ last_x_assum (qspec_then `k` mp_tac)
     \\ simp []
@@ -778,7 +786,7 @@ Proof
   \\ unabbrev_all_tac \\ simp [PULL_EXISTS]
   \\ simp [LNTH_fromList, PULL_EXISTS, GSYM FORALL_AND_THM]
   \\ rpt gen_tac
-  \\ `?a b. evaluate_decs (initial_state ffi k ec) ds1 = (a,b)`
+  \\ `?a b. evaluate_decs (initial_state ffi k ec pe) ds1 = (a,b)`
     by simp [PAIR_FST_SND_EQ]
   \\ fs [eval_sim_def]
   \\ first_x_assum drule
@@ -883,8 +891,8 @@ Proof
 QED
 
 Theorem initial_state_clock:
-  (initial_state ffi k ec).clock = k /\
-  ((initial_state ffi k ec with clock := k1) = initial_state ffi k1 ec)
+  (initial_state ffi k ec pe).clock = k /\
+  ((initial_state ffi k ec pe with clock := k1) = initial_state ffi k1 ec pe)
 Proof
   EVAL_TAC
 QED
@@ -975,7 +983,10 @@ Definition simple_state_rel_def:
         ==> sr (s with globals := sglob) (t with globals := tglob)) /\
     (!s t. sr s t ==> s.ffi = t.ffi) /\
     (!s t sffi tffi. sr s t /\ sffi = tffi
-        ==> sr (s with ffi := sffi) (t with ffi := tffi))
+        ==> sr (s with ffi := sffi) (t with ffi := tffi)) /\
+    (!s t. sr s t ==> s.ptr_eq_oracle = t.ptr_eq_oracle) /\
+    (!s t pe. sr s t
+        ==> sr (s with ptr_eq_oracle := pe) (t with ptr_eq_oracle := pe))
 End
 
 Theorem simple_do_eq_thm_ind:
@@ -1328,6 +1339,14 @@ Proof
     \\ res_tac
     \\ fs [LIST_REL_APPEND_suff, sv_rel_cases, PULL_EXISTS]
     \\ imp_res_tac LIST_REL_LENGTH \\ gvs []
+  )
+  >~ [`Src PtrEq`] >- (
+    rpt strip_tac
+    \\ gvs [do_app_def, AllCaseEqs(), SF DNF_ss]
+    \\ imp_res_tac simple_do_eq_thm
+    \\ `s1.ptr_eq_oracle = s2.ptr_eq_oracle` by fs [simple_state_rel_def]
+    \\ gvs [Boolv_def, simple_val_rel_simps]
+    \\ fs [simple_state_rel_def]
   )
   (* giant mallet for remaining cases *)
   \\ rpt strip_tac
